proofs/core/Substitution.v
@@ -1,0 +1,1289 @@
+Require Import Common.
+Require Import Syntax.
+Require Import Types.
+Require Import Typing.
+Require Import Denotational.
+
+(*Here we define a function to rename bound variables to unique
+  values such that terms and formulas have no duplicate bound
+  variables and no clashes between free and bound variable names.
+  This makes many transformations easier.*)
+
+(*First, some functions we need*)
+
+Definition split {A: Type} (l: list A) (i: nat) : (list A * list A) :=
+  (firstn i l, skipn i l).
+
+(*Split a list into pieces of the appropriate lengths if we can*)
+Fixpoint split_lens {A: Type} (l: list A) (lens: list nat) :
+  list (list A) :=
+  match lens with
+  | len :: tl =>
+    (fst (split l len)) ::
+    split_lens (snd (split l len)) tl
+  | nil => nil
+  end.
+
+Definition sum (l: list nat) : nat :=
+  fold_right (fun x y => x + y) 0 l.
+
+Lemma length_concat {A: Type} (l: list (list A)):
+  length (concat l) = sum (map (@length A) l).
+Proof.
+  induction l; simpl; auto.
+  rewrite app_length, IHl; auto.
+Qed.
+
+Lemma split_lens_length {A: Type} (l: list A) (lens: list nat) :
+  length (split_lens l lens) = length lens.
+Proof.
+  revert l.
+  induction lens; simpl; intros; auto.
+Qed.
+
+Lemma split_lens_concat {A: Type} (l: list A) (lens: list nat) :
+  sum lens = length l ->
+  l = concat (split_lens l lens).
+Proof.
+  revert l. induction lens; simpl; intros; auto.
+  destruct l; auto; inversion H.
+  rewrite <- IHlens.
+  rewrite firstn_skipn; auto.
+  rewrite skipn_length, <- H.
+  rewrite minus_plus; auto.
+Qed.
+
+Lemma split_lens_nodup {A: Type} (l: list A) (lens: list nat) :
+  sum lens = length l ->
+  NoDup l ->
+  forall (i: nat) (d: list A),
+    i < length lens ->
+    NoDup (nth i (split_lens l lens) d).
+Proof.
+  revert l. induction lens; simpl; intros; auto; try lia.
+  destruct i.
+  - apply NoDup_firstn; assumption.
+  - apply IHlens; try lia.
+    + rewrite skipn_length, <- H.
+      rewrite minus_plus; auto.
+    + apply NoDup_skipn; assumption.
+Qed. 
+
+Lemma split_lens_ith {A: Type} (l: list A) (lens: list nat) (i: nat) :
+  sum lens = length l ->
+  i < length lens ->
+  length (nth i (split_lens l lens) nil) = nth i lens 0.
+Proof.
+  revert l i. induction lens; simpl; intros; auto; try lia.
+  destruct i.
+  - rewrite firstn_length.
+    apply Nat.min_l. lia.
+  - specialize (IHlens (skipn a l) i).
+    rewrite IHlens; auto; try lia.
+    rewrite skipn_length, <- H.
+    rewrite minus_plus; auto.
+Qed.
+
+Lemma in_split_lens_ith {A: Type} (l: list A) (lens: list nat) (i: nat) x (d: list A) :
+  sum lens = length l ->
+  i < length lens ->
+  In x (nth i (split_lens l lens) d) ->
+  In x l.
+Proof.
+  revert l i. induction lens; simpl; intros; auto; destruct i; auto; try lia.
+  - apply In_firstn in H1; auto.
+  - apply IHlens in H1; try lia.
+    + apply In_skipn in H1; auto.
+    + rewrite skipn_length, <- H. lia.
+Qed.
+
+Context {sigma: sig}.
+
+
+(*Alpha substitute for patterns only in the given term/formula*)
+(*Here, we need to keep the dependencies between pattern variables
+  (as, for instance, an "or" pattern should have the same free
+  vars on each side, so we use an association list)*)
+  Fixpoint alpha_p_aux {A: Type} (sub: vsymbol -> vsymbol -> A -> A) 
+  (p: pattern) (x: A) (l: list (vsymbol * string)) : (pattern * A) :=
+  match p with
+  | Pvar v => 
+    match (get_assoc_list vsymbol_eq_dec l v) with
+    | Some str => 
+      let v' := (str, snd v) in
+      (Pvar v', sub v v' x)
+    | None => (p, x)
+    end
+  | Pwild => (p, x)
+  | Por p1 p2 =>
+    (*NOTE: must have same free vars*)
+    let t1 := alpha_p_aux sub p1 x l in
+    let t2 := alpha_p_aux sub p2 x l in
+    (Por (fst t1) (fst t2), (snd t2))
+  | Pbind p1 v =>
+    match (get_assoc_list vsymbol_eq_dec l v) with
+    | Some str =>
+      let v' := (str, snd v) in
+      let t := (alpha_p_aux sub p1 x l) in
+      (Pbind (fst t) v', sub v v' (snd t))
+    | None => (p, x)
+    end
+  | Pconstr f tys pats =>
+    let t := 
+    ((fix alpha_ps_aux (l1: list pattern) (y: A) : list pattern * A :=
+      match l1 with
+      | ph :: pt =>
+        let t1 := alpha_p_aux sub ph y l in
+        let t2 := alpha_ps_aux pt (snd t1) in
+        ((fst t1) :: (fst t2), (snd t2))
+      | nil => (nil, y)
+      end) pats x) in
+    (Pconstr f tys (fst t), (snd t))
+    end.
+(*Proving this correct will not be too fun, but let's see*)
+
+Fixpoint alpha_t_aux (t: term) (l: list string) {struct t} : term :=
+  (*We only care about the bound variable and inductive cases*)
+  match t with
+  | Tlet t1 x t2 => 
+    match l with
+    | str :: tl =>
+      let (l1, l2) := split tl (length (bnd_t t1)) in 
+      Tlet (alpha_t_aux t1 l1) (str, snd x) (sub_t x (str, snd x) 
+      (alpha_t_aux t2 l2))
+    | _ => t
+    end
+  | Tfun fs tys tms =>
+    (*Split up the list into pieces of appropriate lengths 
+      (size (bnd_t tm))*)
+    let lens := map (fun tm => length (bnd_t tm)) tms in
+    let l_split := split_lens l lens in
+    Tfun fs tys (map2 (fun (tm: term) (l': list string) =>
+    alpha_t_aux tm l') tms l_split)
+  | Tif f t1 t2 =>
+    let f_sz := length (bnd_f f) in
+    let t1_sz := length (bnd_t t1) in
+    let (l1, lrest) := split l f_sz in
+    let (l2, l3) := split lrest t1_sz in
+    Tif (alpha_f_aux f l1) 
+      (alpha_t_aux t1 l2)
+      (alpha_t_aux t2 l3)
+  | Tmatch t1 ty ps =>
+    (*First do the pattern substitutions, then do the terms
+      recursively*)
+    let lens := map (fun x => length (pat_fv (fst x)) + 
+      length (bnd_t (snd x))) ps in
+    let t1_sz := length (bnd_t t1) in
+    let (l1, l2) := split l (t1_sz) in
+    let l_split := split_lens l2 lens in
+    
+    Tmatch (alpha_t_aux t1 l1) ty
+      (map2 (fun (x: pattern * term) (strs: list string) =>
+        let p_sz := length (pat_fv (fst x)) in
+        let (l1, l2) := split strs p_sz in
+        let t2 := alpha_t_aux (snd x) l2 in
+        alpha_p_aux sub_t (fst x) t2  (combine (pat_fv (fst x)) l1)
+        ) ps l_split)
+  | Teps f v =>
+    match l with
+    | nil => t
+    | str :: tl =>
+      let v' := (str, snd v) in
+      Teps (sub_f v v' (alpha_f_aux f tl)) v'
+    end
+  | _ => t (*no other bound variables/recursive cases*)
+  end
+with alpha_f_aux (f: formula) (l: list string) {struct f} : formula :=
+  match f with
+  | Fpred ps tys tms =>
+    (*Split up the list into pieces of appropriate lengths 
+      (size (bnd_t tm))*)
+    let lens := map (fun tm => length (bnd_t tm)) tms in
+    let l_split := split_lens l lens in
+    Fpred ps tys (map2 (fun (t: term) (l': list string) =>
+      alpha_t_aux t l') tms l_split)
+  | Fquant q v f1 =>
+      match l with
+      | str :: tl =>
+        let v' := (str, snd v) in
+        Fquant q v' (sub_f v v' (alpha_f_aux f1 tl))
+      | _ => f
+      end
+  | Feq ty t1 t2 =>
+    let t_sz := length (bnd_t t1) in
+    let (l1, l2) := split l t_sz in
+    Feq ty (alpha_t_aux t1 l1)
+      (alpha_t_aux t2 l2)
+  | Fbinop b f1 f2 =>
+    let f_sz := length (bnd_f f1) in
+    let (l1, l2) := split l f_sz in
+    Fbinop b (alpha_f_aux f1 l1)
+      (alpha_f_aux f2 l2)
+  | Fnot f1 =>
+    Fnot (alpha_f_aux f1 l)
+  | Flet t v f1 =>
+    match l with
+    | str :: tl =>
+      let (l1, l2) := split tl (length (bnd_t t)) in 
+      Flet (alpha_t_aux t l1) (str, snd v) (sub_f v (str, snd v) 
+      (alpha_f_aux f1 l2))
+    | _ => f
+    end
+  | Fif f1 f2 f3 =>
+    let f1_sz := length (bnd_f f1) in
+    let f2_sz := length (bnd_f f2) in
+    let (l1, lrest) := split l f1_sz in
+    let (l2, l3) := split lrest f2_sz in
+    Fif (alpha_f_aux f1 l1) 
+      (alpha_f_aux f2 l2)
+      (alpha_f_aux f3 l3)
+  | Fmatch t1 ty ps =>
+    (*First do the pattern substitutions, then do the terms
+      recursively*)
+    let lens := map (fun x => length (pat_fv (fst x)) + 
+    length (bnd_f (snd x))) ps in
+    let t1_sz := length (bnd_t t1) in
+    let (l1, l2) := split l t1_sz in
+    let l_split := split_lens l2 lens in
+    
+    Fmatch (alpha_t_aux t1 l1) ty
+      (map2 (fun (x: pattern * formula) (strs: list string) =>
+        let p_sz := length (pat_fv (fst x)) in
+        let (l1, l2) := split strs p_sz in
+        let f2 := alpha_f_aux (snd x) l2 in
+        alpha_p_aux sub_f (fst x) f2  (combine (pat_fv (fst x)) l1)
+        ) ps l_split)
+  | _ => f (*No other bound/recursive cases*)
+  end.
+(*Prove correctness: 3 lemmas
+  1. results in wf term/fmla
+  2. preserves interp
+  3. has same "shape" (and corollaries: ind form, positive, etc)*)
+
+
+Lemma NoDup_pat_fv (p: pattern) : NoDup (pat_fv p).
+Proof.
+  induction p; simpl; try constructor; auto.
+  - constructor.
+  - apply big_union_nodup.
+  - apply union_nodup; auto.
+  - apply union_nodup; auto. constructor; auto. constructor.
+Qed.
+
+(*TODO: see if we need*)
+Lemma alpha_p_aux_wf_aux_gen {A: Type} (p: pattern) 
+  (sub: vsymbol -> vsymbol -> A -> A) :
+  (forall (l: list (vsymbol * string)),
+    (*NoDup (map snd l) ->*)
+    (forall v, In v (pat_fv p) -> In v (map fst l)) ->
+    (*NoDup (map fst l) ->*)
+    (forall x v, In v (pat_fv (fst (alpha_p_aux sub p x l))) ->
+      exists v', In (v', (fst v)) l /\
+        In v' (pat_fv p))).
+Proof.
+  intros l (*Hnodups*) Hfvs (*Hnodupf*).
+  induction p; simpl; auto; intros.
+  - destruct (get_assoc_list vsymbol_eq_dec l v) eqn : Ha.
+    + simpl in H. destruct H as [Heq | []]; subst; simpl.
+      apply get_assoc_list_some in Ha.
+      exists v. auto.
+    + apply get_assoc_list_none in Ha. simpl in H.
+      destruct H as [Heq | []]; subst.
+      exfalso. apply Ha. apply (Hfvs v0); auto. simpl; auto.
+  - generalize dependent x. induction ps; simpl in *; auto; intros. 
+    destruct H0.
+    inversion H; subst.
+    rewrite union_elts in H0. destruct H0.
+    + assert (Hv: exists v', In (v', fst v) l /\ In v' (pat_fv a)). {
+        apply H3 with(x:=x); auto. intros. apply Hfvs.
+        rewrite union_elts. left; auto.
+      }
+      destruct Hv as [v' [Hinl Hinv']].
+      exists v'. split; auto. rewrite union_elts. left; auto.
+    + assert (Hv: exists v' : vsymbol,
+        In (v', fst v) l /\ In v' (big_union vsymbol_eq_dec pat_fv ps)). {
+        apply IHps with (x:=(snd (alpha_p_aux sub a x l))); auto.
+        intros. apply Hfvs. rewrite union_elts. right; auto.
+      }
+      destruct Hv as [v' [Hinl Hinv']]; subst.
+      exists v'. split; auto. rewrite union_elts. right; auto.
+  - destruct H.
+  - rewrite union_elts in H.
+    destruct H.
+    + assert (Hv: exists v' : vsymbol, In (v', fst v) l /\ In v' (pat_fv p1)). {
+        apply IHp1 with(x:=x); auto. intros. apply Hfvs; simpl;
+        rewrite union_elts; left; auto.
+      }
+      destruct Hv as [v' [Hinl Hinv']].
+      exists v'. split; auto. rewrite union_elts. left; auto.
+    + assert (Hv: exists v' : vsymbol, In (v', fst v) l /\ In v' (pat_fv p2)). {
+        apply IHp2 with(x:=x); auto.
+        intros; apply Hfvs; simpl; rewrite union_elts; right; auto.
+      } destruct Hv as [v' [Hinl Hinv']]; subst.
+      exists v'. split; auto. rewrite union_elts; right; auto. 
+  - destruct (get_assoc_list vsymbol_eq_dec l v) eqn : Ha.
+    + simpl in H. rewrite union_elts in H.
+      destruct H as [Hinv | [Heq | []]]; subst.
+      * apply IHp with(x:=x) in Hinv.
+        destruct Hinv as [v' [Hl Hv']].
+        exists v'; split; auto. rewrite union_elts; left; auto.
+        intros. apply Hfvs; simpl; rewrite union_elts; left; auto.
+      * apply get_assoc_list_some in Ha.
+        exists v. split; auto. rewrite union_elts; right; auto.
+        left; auto.
+    + simpl in H. apply get_assoc_list_none in Ha.
+      exfalso. apply Ha. apply Hfvs. simpl. auto.
+      rewrite union_elts. right; left; auto.
+Qed. 
+
+(*Other direction*)
+Lemma alpha_p_aux_wf_aux_gen' {A: Type} (p: pattern) 
+  (sub: vsymbol -> vsymbol -> A -> A) :
+  (forall (l: list (vsymbol * string)),
+    NoDup (map fst l) ->
+    (forall v, In v (pat_fv p) -> In v (map fst l)) ->
+    (forall x d, 
+      In x (pat_fv (fst (alpha_p_aux sub p d l))) <->
+      exists v str, 
+        In (v, str) l /\
+        In v (pat_fv p) /\
+        snd x = snd v /\
+        fst x = str)).
+Proof.
+  intros l Hnodup Hfvs (*Hnodupf*).
+  induction p; simpl; auto; intros.
+  - destruct (get_assoc_list vsymbol_eq_dec l v) eqn : Ha; simpl; split; intros.
+    + destruct H as [Heq | []]; subst; simpl.
+      apply get_assoc_list_some in Ha.
+      exists v. exists s. split; auto.
+    + destruct H as [v1 [str [Hinl [[Heq | []] [Hsnd Hfst]]]]]; subst.
+      left. destruct x; simpl in *; subst.
+      f_equal. symmetry.
+      apply get_assoc_list_some in Ha. 
+      apply (nodup_fst_inj Hnodup Hinl Ha).
+    + apply get_assoc_list_none in Ha.
+      destruct H as [Heq | []]; subst.
+      exfalso. apply Ha. apply Hfvs. left; auto.
+    + apply get_assoc_list_none in Ha.
+      destruct H as [v1 [str [Hinl [[Heq | []] [Hsnd Hfst]]]]]; subst.
+      exfalso. apply Ha. rewrite in_map_iff. exists (v1, fst x); auto.
+  - generalize dependent d. induction ps; simpl in *; auto; intros; 
+    [split; simpl; intros; auto |].
+    + destruct H0.
+    + destruct H0 as [v1 [str [Hinl [[] _]]]].
+    + assert (Hfvs': (forall v : vsymbol,
+      In v (big_union vsymbol_eq_dec pat_fv ps) -> In v (map fst l))).
+      {
+        intros; apply Hfvs; simpl; rewrite union_elts; right; auto.
+      } inversion H; subst. split; simpl; intros; auto.  
+      rewrite union_elts in H0. inversion H; subst.
+      destruct H0.
+      * apply H2 in H0; auto.
+        destruct H0 as [v1 [str [Hinl [Hinv [Hsnd Hfst]]]]]; subst.
+        exists v1. exists (fst x). split_all; auto.
+        rewrite union_elts; left; auto.
+        intros. apply Hfvs. rewrite union_elts. left; auto.
+      * specialize (IHps H3 Hfvs' (snd (alpha_p_aux sub a d l))).
+        apply IHps in H0; clear IHps.
+        destruct H0 as [v1 [str [Hinl [Hinv [Hsnd Hfst]]]]]; subst.
+        exists v1. exists (fst x). split_all; auto.
+        rewrite union_elts. right; auto.
+      * destruct H0 as [v1 [str [Hinl [Hinv [Hsnd Hfst]]]]]; subst.
+        rewrite union_elts in Hinv.
+        rewrite union_elts.
+        destruct Hinv as [Hinv1 | Hinv1]; [left | right].
+        -- apply H2; auto. intros; apply Hfvs; simpl; rewrite union_elts;
+          left; auto.
+          exists v1. exists (fst x). auto.
+        -- apply IHps; auto.
+          exists v1. exists (fst x). auto.
+  - split; intros; auto. destruct H. 
+    destruct H as [_ [_ [_ [[] _]]]].
+  - rewrite union_elts. split; intros.
+    + destruct H; [apply IHp1 in H | apply IHp2 in H];
+      try (intros; apply Hfvs; simpl; rewrite union_elts;
+        try(solve[left; auto]); right; auto);
+      destruct H as [v1 [str [Hinl [Hinv [Hsnd Hfst]]]]]; subst;
+      exists v1; exists (fst x); split_all; auto;
+      rewrite union_elts; [left | right]; auto.
+    + destruct H as [v1 [str [Hinl [Hinv [Hsnd Hfst]]]]]; subst.
+      rewrite union_elts in Hinv. destruct Hinv; 
+      [left; apply IHp1 | right; apply IHp2]; try (intros; apply Hfvs;
+      simpl; rewrite union_elts; try(solve[left; auto]); right; auto);
+      exists v1; exists (fst x); split_all; auto.
+  - destruct (get_assoc_list vsymbol_eq_dec l v) eqn : Ha; simpl;
+    rewrite union_elts; [split; intros|].
+    + destruct H as [Hinx | [Heq | []]]; subst.
+      * apply IHp in Hinx.
+        destruct Hinx as [v1 [str [Hinl [Hinv [Hsnd Hfst]]]]]; subst.
+        exists v1. exists (fst x). split_all; auto.
+        rewrite union_elts; left; auto.
+        intros; apply Hfvs; simpl; rewrite union_elts; left; auto.
+      * apply get_assoc_list_some in Ha.
+        exists v. exists s. split_all; auto. rewrite union_elts.
+        right; left;auto.
+    + destruct H as [v1 [str [Hinl [Hinv [Hsnd Hfst]]]]]; subst.
+      rewrite union_elts in Hinv. destruct Hinv as [Hinv | [Heq | []]]; subst;
+      [left | right; left]; auto.
+      * apply IHp. intros. apply Hfvs; simpl; rewrite union_elts; left; auto.
+        exists v1. exists (fst x). split_all; auto.
+      * apply get_assoc_list_some in Ha.
+        destruct x; simpl in *; subst. f_equal.
+        apply (nodup_fst_inj Hnodup Ha Hinl).
+    + apply get_assoc_list_none in Ha.
+      exfalso. apply Ha. apply Hfvs. simpl. rewrite union_elts; right; left;
+      auto.
+Qed.
+
+Lemma alpha_p_aux_wf_aux {A: Type} (p: pattern) 
+  (sub: vsymbol -> vsymbol -> A -> A) :
+  (forall (l: list (vsymbol * string)),
+    NoDup (map fst l) ->
+    (forall v, In v (pat_fv p) -> In v (map fst l)) ->
+    (forall x v, In v (pat_fv (fst (alpha_p_aux sub p x l))) ->
+      In (fst v) (map snd l))).
+Proof.
+  intros. pose proof (alpha_p_aux_wf_aux_gen' p sub l H H0 v x).
+  apply H2 in H1. destruct H1 as [v1 [str [Hinl [Hinv1 [Hsnd Hfst]]]]]; subst.
+  rewrite in_map_iff. exists (v1, fst v). split; auto.
+Qed.
+
+(*Second: need to know that [alpha_p_aux] does not change any bound
+  variables in t/f*)
+
+Lemma alpha_p_aux_bnd_t_eq  (p: pattern) (t: term) (l: list (vsymbol * string)) :
+  bnd_t (snd (alpha_p_aux sub_t p t l)) =
+  bnd_t t.
+Proof.
+  revert t.
+  induction p; simpl; intros; auto.
+  - destruct (get_assoc_list vsymbol_eq_dec l v); simpl; auto.
+    rewrite bnd_sub_t; auto.
+  - generalize dependent t. induction ps; simpl; intros; auto. 
+    inversion H; subst.
+    rewrite IHps; auto.
+  - destruct (get_assoc_list vsymbol_eq_dec l v); simpl; auto.
+    rewrite bnd_sub_t; auto.
+Qed.
+
+Lemma alpha_p_aux_bnd_f_eq (p: pattern) (f: formula) (l: list (vsymbol * string)) :
+  bnd_f (snd (alpha_p_aux sub_f p f l)) =
+  bnd_f f.
+Proof.
+  revert f.
+  induction p; simpl; intros; auto.
+  - destruct (get_assoc_list vsymbol_eq_dec l v); simpl; auto.
+    rewrite bnd_sub_f; auto.
+  - generalize dependent f0. induction ps; simpl; intros; auto. 
+    inversion H; subst.
+    rewrite IHps; auto.
+  - destruct (get_assoc_list vsymbol_eq_dec l v); simpl; auto.
+    rewrite bnd_sub_f; auto.
+Qed.
+
+(*TODO: add to this*)
+(*Solve trivial/repeated goals and simplify*)
+Ltac len_tac :=
+repeat match goal with
+| |- context [length (firstn ?n ?l)] => rewrite firstn_length
+| |- context [length (skipn ?n ?l)] => rewrite skipn_length
+| H: length ?l = ?x |- context [length ?l] => rewrite H
+| |- context [length (?x ++ ?y)] => rewrite app_length
+end; try lia.
+
+Ltac wf_tac :=
+  repeat(
+  assumption +
+  solve[len_tac] +
+  solve[lia] +
+  match goal with
+  | |- context [map snd (combine ?l1 ?l2)] =>
+    rewrite map_snd_combine
+  | |- context [map fst (combine ?l1 ?l2)] =>
+    rewrite map_fst_combine
+  | |- NoDup (firstn ?n ?l) => apply NoDup_firstn
+  | |- NoDup (skipn ?n ?l) => apply NoDup_skipn
+  | |- NoDup (nth ?i (split_lens ?a ?b) ?d) =>
+    apply split_lens_nodup
+  | |- context [length (map ?f ?x)] => rewrite map_length
+  | |- context [length (split_lens ?l1 ?l2)] =>
+    rewrite split_lens_length
+  | |- context [length (firstn ?n ?l)] => rewrite firstn_length
+  | |- context [length (skipn ?n ?l)] => rewrite skipn_length
+  | |- In (nth ?i ?l ?x) ?l =>
+    apply nth_In
+  | |- context [length (nth ?l (split_lens ?a ?b) ?d)] =>
+    rewrite split_lens_ith
+  | |- context [length (map2 ?f ?l1 ?l2)] =>
+    rewrite map2_length
+  | |- ?i < length ?l -> ?P => intros
+  | |- context [Nat.min ?x ?x] =>
+    rewrite Nat.min_id
+  (*TODO: this is hacky*)
+  | |- context [nth ?i (map ?f ?l) ?d] =>
+    (rewrite map_nth_inbound with(d2:=tm_d)) ||
+    (rewrite map_nth_inbound with (d2:=(Pwild, tm_d))) ||
+    (rewrite map_nth_inbound with (d2:=(Pwild, Ftrue)))
+  (*Deal with some "In" goals - TODO improve*)
+  | H: In ?x (firstn ?n ?l) |- In ?x ?l => apply In_firstn in H
+  | H: In ?x (skipn ?n ?l) |- In ?x ?l => apply In_skipn in H
+  (*A special case*)
+  | |- NoDup (pat_fv ?p) => apply NoDup_pat_fv
+  | |- context [concat (split_lens ?l1 ?l2)] =>
+    rewrite <- split_lens_concat
+  | |- In ?x (map ?g ?l) => rewrite in_map_iff
+  | |- exists y, ?f y = ?f ?x /\ ?P => exists x; split
+  (*Solve the sum length goal*)
+  | H: length ?l = length (concat (map ?f ?l1)) |-
+    sum (map ?g ?l1) = length ?l => rewrite length_concat in H;
+    rewrite H; f_equal; rewrite map_map; apply map_ext
+  | H: length (?x :: ?l) = ?n |- _ => simpl in H
+  | H: ?x = length (?l1 ++ ?l2) |- _ => rewrite app_length in H
+  end); auto; try lia. 
+
+Lemma alpha_aux_wf_aux (t: term) (f: formula) :
+  (forall (l: list string),
+    NoDup l ->
+    length l = length (bnd_t t) ->
+    NoDup (bnd_t (alpha_t_aux t l)) /\
+    (forall x, In x (bnd_t (alpha_t_aux t l)) -> In (fst x) l)) /\
+  (forall (l: list string),
+    NoDup l ->
+    length l = length (bnd_f f) ->
+    NoDup (bnd_f (alpha_f_aux f l)) /\
+    (forall x, In x (bnd_f (alpha_f_aux f l)) -> In (fst x) l)).
+Proof.
+  revert t f.
+  apply term_formula_ind; simpl; intros; auto.
+  - split; [constructor | intros x []]. 
+  - split; [constructor | intros x []].
+  - (*Tfun case*) 
+    split.
+    + rewrite NoDup_concat_iff. split.
+      * intros x. rewrite in_map_iff.
+        intros [t1 [Hbndt1 Hint1]]. subst.
+        rewrite in_map2_iff with(d1:=tm_d)(d2:=nil) in Hint1;
+        wf_tac.
+        destruct Hint1 as [i [Hi Ht1]]; subst.
+        rewrite Forall_forall in H.
+        apply H; simpl; wf_tac.
+      * intros i1 i2 d x. wf_tac.
+        intros [Hin1 Hin2].
+        (*Idea: suppose in both, then by IH (twice), in 2 different
+          parts of l - contradicts NoDup l*)
+        rewrite Forall_forall in H.
+        rewrite (map2_nth _ _ _ tm_d nil) in Hin1, Hin2; wf_tac.
+        apply H in Hin1, Hin2; auto; wf_tac.
+        assert (NoDup (concat (split_lens l0 (map (fun t => length (bnd_t t)) l1)))) by
+          (rewrite <- split_lens_concat; wf_tac).
+          rewrite NoDup_concat_iff in H5.
+        split_all. apply (H6 i1 i2 nil (fst x)); wf_tac.
+    + intros x. rewrite in_concat. intros [bl [Hinbl Hinx]].
+      rewrite in_map_iff in Hinbl.
+      destruct Hinbl as [t1 [Ht1 Hint1]]; subst.
+      rewrite (in_map2_iff _ _ _ tm_d nil) in Hint1; wf_tac.
+      destruct Hint1 as [i [Hi Ht1]]; subst.
+      rewrite Forall_forall in H.
+      apply H in Hinx; auto; wf_tac.
+      rewrite (split_lens_concat l0 (map (fun t => length (bnd_t t)) l1));
+      [|wf_tac]. rewrite in_concat. eexists. split; [| apply Hinx]. wf_tac.
+  - (*Tlet case*)
+    destruct l; inversion H2; simpl.
+    inversion H1; subst.
+    split.
+    + constructor.
+      * (*TODO: automate the "In" part*) 
+        intro Hin.
+        apply in_app_or in Hin.
+        destruct Hin.
+        -- apply H in H3; wf_tac.
+          apply In_firstn in H3. contradiction.
+        -- rewrite bnd_sub_t in H3.
+          apply H0 in H3; wf_tac. apply In_skipn in H3.
+          contradiction.
+      * rewrite NoDup_app_iff'.
+        split_all.
+        -- apply H; wf_tac.
+        -- rewrite bnd_sub_t. apply H0; wf_tac.
+        -- intros x.
+          rewrite bnd_sub_t.
+          intros [Hinx1 Hinx2].
+          apply H in Hinx1; wf_tac.
+          apply H0 in Hinx2; wf_tac.
+          apply (nodup_firstn_skipn Hinx1 Hinx2); auto.
+    + intros x [Hx | Hinx]; subst;[left; auto|].
+      apply in_app_or in Hinx.
+      destruct Hinx as [Hinx | Hinx].
+      * apply H in Hinx; wf_tac.
+        right. apply In_firstn in Hinx; auto.
+      * rewrite bnd_sub_t in Hinx. apply H0 in Hinx; wf_tac.
+        right. apply In_skipn in Hinx; auto.
+  - (*Tif case*)
+    split.
+    + rewrite !NoDup_app_iff'.
+      split_all.
+      * apply H; wf_tac.
+      * apply H0; wf_tac.
+      * apply H1; wf_tac.
+      * intros x [Hinx1 Hinx2].
+        apply H0 in Hinx1; wf_tac.
+        apply H1 in Hinx2; wf_tac.
+        apply (nodup_firstn_skipn Hinx1 Hinx2); wf_tac. 
+      * intros x [Hinx1 Hinx2].
+        apply H in Hinx1; wf_tac.
+        apply in_app_or in Hinx2. destruct Hinx2.
+        -- apply H0 in H4; wf_tac.
+          apply (nodup_firstn_skipn Hinx1); wf_tac. 
+        -- apply H1 in H4; wf_tac.
+          apply (nodup_firstn_skipn Hinx1); wf_tac.
+    + intros x Hinx.
+      repeat (apply in_app_or in Hinx; destruct Hinx as [Hinx | Hinx]).
+      * apply H in Hinx; wf_tac.
+      * apply H0 in Hinx; wf_tac. apply In_firstn in Hinx.
+        apply In_skipn in Hinx; auto.
+      * apply H1 in Hinx; wf_tac. apply In_skipn in Hinx.
+        apply In_skipn in Hinx; auto.
+  - (*Tmatch case*)
+    assert (Hsum: sum (map
+        (fun x : pattern * term =>
+        Datatypes.length (pat_fv (fst x)) + Datatypes.length (bnd_t (snd x)))
+        ps) = Datatypes.length (skipn (Datatypes.length (bnd_t tm)) l)). {
+          wf_tac. rewrite H2,length_concat, 
+        map_map, minus_plus. f_equal. apply map_ext_in_iff; intros.
+        rewrite app_length; auto.
+    }
+    split.
+    + rewrite NoDup_app_iff'; split_all.
+      * apply H; wf_tac.
+      * rewrite NoDup_concat_iff; split_all.
+        -- intros x. rewrite in_map_iff.
+          intros [pt1 [Hx Hinx]]; subst.
+          rewrite (in_map2_iff _ _ _ (Pwild, tm_d) nil) in Hinx; wf_tac.
+          destruct Hinx as [i [Hi Hpt1]].
+          rewrite NoDup_app_iff'.
+          split_all; subst; wf_tac.
+          ++ rewrite alpha_p_aux_bnd_t_eq.
+            rewrite Forall_forall in H0.
+            apply H0; auto; wf_tac.
+          ++ intros x.
+            rewrite alpha_p_aux_bnd_t_eq.
+            intros [Hinx1 Hinx2].
+            (*Need this a lot even though it's ugly*)
+            apply alpha_p_aux_wf_aux in Hinx1; wf_tac.
+            rewrite map_snd_combine in Hinx1; wf_tac.
+            rewrite Forall_forall in H0.
+            apply H0 in Hinx2; wf_tac.
+            apply (nodup_firstn_skipn Hinx1 Hinx2); wf_tac.
+        -- intros i1 i2 d x. wf_tac.
+          rewrite !map2_nth with(d1:=(Pwild, tm_d)) (d2:=nil); wf_tac.
+          intros [Hini1 Hini2].
+          apply in_app_or in Hini1, Hini2.
+          (*Now we get 4 cases need to show each is impossible*)
+          destruct Hini1 as [Hini1 | Hini1].
+          ++ apply alpha_p_aux_wf_aux in Hini1; wf_tac.
+            revert Hini1. wf_tac. intros Hini1.
+            apply In_firstn in Hini1.
+            destruct Hini2 as [Hini2 | Hini2].
+            ** apply alpha_p_aux_wf_aux in Hini2; wf_tac.
+              revert Hini2. wf_tac. intros Hini2.
+              apply In_firstn in Hini2.
+              apply H5.
+              apply (in_nth_concat_nodup Hini1 Hini2); wf_tac.
+            ** rewrite alpha_p_aux_bnd_t_eq in Hini2.
+              rewrite Forall_forall in H0.
+              apply H0 in Hini2; wf_tac.
+              apply In_skipn in Hini2.
+              apply H5.
+              apply (in_nth_concat_nodup Hini1 Hini2); wf_tac.
+          ++ rewrite alpha_p_aux_bnd_t_eq in Hini1.
+            rewrite Forall_forall in H0.
+            apply H0 in Hini1; wf_tac.
+            apply In_skipn in Hini1.
+            destruct Hini2 as [Hini2 | Hini2].
+            ** apply alpha_p_aux_wf_aux in Hini2; wf_tac.
+              revert Hini2; wf_tac. intros Hini2.
+              apply In_firstn in Hini2.
+              apply H5.
+              apply (in_nth_concat_nodup Hini1 Hini2); wf_tac.
+            ** rewrite alpha_p_aux_bnd_t_eq in Hini2.
+              apply H0 in Hini2; wf_tac.
+              apply In_skipn in Hini2.
+              apply H5.
+              apply (in_nth_concat_nodup Hini1 Hini2); wf_tac.
+      * intros x.
+        rewrite in_concat. intros [Hinx1 [l1 [Hinl1 Hinxl1]]].
+        apply H in Hinx1; wf_tac.
+        rewrite in_map_iff in Hinl1. destruct Hinl1 as [p1 [Hl1 Hinp1]].
+        subst.
+        rewrite in_map2_iff with(d1:=(Pwild, tm_d))(d2:=nil) in Hinp1; wf_tac.
+        destruct Hinp1 as [i [Hi Hp1]]; subst.
+        (*And now we have to show these are distinct, will be similar*)
+        apply in_app_or in Hinxl1.
+        destruct Hinxl1 as [Hinx2 | Hinx2].
+        -- apply alpha_p_aux_wf_aux in Hinx2; wf_tac.
+          revert Hinx2; wf_tac; intros.
+          apply In_firstn in Hinx2.
+          apply in_split_lens_ith in Hinx2; wf_tac.
+          apply (nodup_firstn_skipn Hinx1 Hinx2); wf_tac.
+        -- rewrite alpha_p_aux_bnd_t_eq in Hinx2.
+          rewrite Forall_forall in H0; apply H0 in Hinx2; wf_tac.
+          apply In_skipn in Hinx2.
+          apply in_split_lens_ith in Hinx2; wf_tac.
+          apply (nodup_firstn_skipn Hinx1 Hinx2); wf_tac.
+    + (*Second part - TODO very similar to previous*)
+      intros x Hinx.
+      apply in_app_or in Hinx.
+      destruct Hinx as [Hinx | Hinx].
+      * apply H in Hinx; wf_tac.
+      * rewrite in_concat in Hinx.
+        destruct Hinx as [l1 [Hinl1 Hinxl1]].
+        rewrite in_map_iff in Hinl1.
+        destruct Hinl1 as [p1 [Hl1 Hinp1]].
+        subst.
+        rewrite in_map2_iff with (d1:=(Pwild, tm_d))(d2:=nil) in Hinp1; wf_tac.
+        destruct Hinp1 as [i [Hi Hp1]]; subst.
+        apply in_app_or in Hinxl1.
+        destruct Hinxl1 as [Hinx | Hinx].
+        -- apply alpha_p_aux_wf_aux in Hinx; wf_tac.
+          revert Hinx; wf_tac; intros.
+          apply In_firstn in Hinx.
+          apply in_split_lens_ith in Hinx; wf_tac.
+        -- rewrite alpha_p_aux_bnd_t_eq in Hinx.
+          rewrite Forall_forall in H0; apply H0 in Hinx; wf_tac.
+          apply In_skipn in Hinx.
+          apply in_split_lens_ith in Hinx; wf_tac.
+  - (*Epsilon case*)
+    destruct l; inversion H1; subst; simpl.
+    inversion H0; subst.
+    rewrite bnd_sub_f.
+    split.
+    + constructor; [|apply H; wf_tac].
+      intro Hin. apply H in Hin; wf_tac.
+    + intros. destruct H2; subst; [left; auto | right].
+      apply H in H2; wf_tac.
+  - (*Fpred case - same as Tfun*)
+    split.
+    + rewrite NoDup_concat_iff. split.
+      * intros x. rewrite in_map_iff.
+        intros [t1 [Hbndt1 Hint1]]. subst.
+        rewrite in_map2_iff with(d1:=tm_d)(d2:=nil) in Hint1;
+        wf_tac.
+        destruct Hint1 as [i [Hi Ht1]]; subst.
+        rewrite Forall_forall in H.
+        apply H; simpl; wf_tac.
+      * intros i1 i2 d x. wf_tac.
+        intros [Hin1 Hin2].
+        (*Idea: suppose in both, then by IH (twice), in 2 different
+          parts of l - contradicts NoDup l*)
+        rewrite Forall_forall in H.
+        rewrite (map2_nth _ _ _ tm_d nil) in Hin1, Hin2; wf_tac.
+        apply H in Hin1, Hin2; auto; wf_tac.
+        assert (NoDup (concat (split_lens l (map (fun t => length (bnd_t t)) tms)))) by
+          (rewrite <- split_lens_concat; wf_tac).
+          rewrite NoDup_concat_iff in H5.
+        split_all. apply (H6 i1 i2 nil (fst x)); wf_tac.
+    + intros x. rewrite in_concat. intros [bl [Hinbl Hinx]].
+      rewrite in_map_iff in Hinbl.
+      destruct Hinbl as [t1 [Ht1 Hint1]]; subst.
+      rewrite (in_map2_iff _ _ _ tm_d nil) in Hint1; wf_tac.
+      destruct Hint1 as [i [Hi Ht1]]; subst.
+      rewrite Forall_forall in H.
+      apply H in Hinx; auto; wf_tac.
+      rewrite (split_lens_concat l (map (fun t => length (bnd_t t)) tms));
+        [|wf_tac]. rewrite in_concat. eexists. split; [| apply Hinx]. wf_tac.
+  - (*Fquant*)
+    destruct l; inversion H1; subst; simpl.
+    inversion H0; subst.
+    rewrite bnd_sub_f.
+    split.
+    + constructor; [intro C; apply H in C |apply H]; wf_tac.
+    + intros. destruct H2; subst;[left | right]; auto.
+      apply H in H2; wf_tac.
+  - (*Feq*)
+    split.
+    + rewrite NoDup_app_iff'; split_all;[apply H | apply H0 |]; wf_tac.
+      intros x [Hinx1 Hinx2].
+      apply H in Hinx1; wf_tac; apply H0 in Hinx2; wf_tac.
+      apply (nodup_firstn_skipn Hinx1); wf_tac.
+    + intros x Hinx.
+      apply in_app_or in Hinx. destruct Hinx as [Hinx | Hinx]; 
+      [apply H in Hinx | apply H0 in Hinx];wf_tac.
+  - (*Fbinop*)
+    split.
+    + rewrite NoDup_app_iff'; split_all;[apply H|apply H0|]; wf_tac.
+      intros x [Hinx1 Hinx2].
+      apply H in Hinx1; wf_tac; apply H0 in Hinx2; wf_tac.
+      apply (nodup_firstn_skipn Hinx1); wf_tac.
+    + intros x Hinx.
+      apply in_app_or in Hinx; destruct Hinx as [Hinx | Hinx];
+      [apply H in Hinx | apply H0 in Hinx];wf_tac.
+  - (*trivial*)
+    split;[constructor | intros x []].
+  - split;[constructor | intros x []].
+  - (*Flet*)
+    destruct l; inversion H2; subst.
+    inversion H1; subst; simpl; rewrite bnd_sub_f.
+    split.
+    + constructor.
+      * intro C. apply in_app_or in C.
+        destruct C as [Hins | Hins];
+        [apply H in Hins | apply H0 in Hins]; wf_tac;
+        [apply In_firstn in Hins | apply In_skipn in Hins];
+        contradiction.
+      * rewrite NoDup_app_iff'; split_all; [apply H | apply H0 |];wf_tac.
+        intros x [Hinx1 Hinx2]; apply H in Hinx1; apply H0 in Hinx2; wf_tac.
+        apply (nodup_firstn_skipn Hinx1); wf_tac.
+    + intros x [Hx | Hinx]; subst;[left | right]; auto.
+      apply in_app_or in Hinx; destruct Hinx as [Hinx | Hinx];
+      [apply H in Hinx | apply H0 in Hinx]; wf_tac.
+  - (*Fif*)
+    split.
+    + rewrite !NoDup_app_iff'; split_all;
+      [apply H | apply H0 | apply H1 | |]; wf_tac;
+      intros x; [| rewrite in_app_iff];
+      intros [Hinx1 Hinx2];[|destruct Hinx2 as [Hinx2 | Hinx2]];
+      [apply H0 in Hinx1; apply H1 in Hinx2 | apply H in Hinx1; 
+        apply H0 in Hinx2 | apply H in Hinx1; apply H1 in Hinx2]; wf_tac;
+      apply (nodup_firstn_skipn Hinx1); wf_tac.
+    + intros x.
+      rewrite ! in_app_iff; intros [Hinx | [Hinx | Hinx]];
+      [apply H in Hinx | apply H0 in Hinx | apply H1 in Hinx]; wf_tac.
+      * apply In_firstn in Hinx. wf_tac.
+      * apply In_skipn in Hinx. wf_tac.
+  - (*Fmatch case - very similar to Tmatch*)
+    assert (Hsum: sum (map
+      (fun x : pattern * formula =>
+      Datatypes.length (pat_fv (fst x)) + Datatypes.length (bnd_f (snd x)))
+      ps) = Datatypes.length (skipn (Datatypes.length (bnd_t tm)) l)). {
+        wf_tac. rewrite H2,length_concat, 
+      map_map, minus_plus. f_equal. apply map_ext_in_iff; intros.
+      rewrite app_length; auto.
+    }
+    split.
+    + rewrite NoDup_app_iff'; split_all.
+      * apply H; wf_tac.
+      * rewrite NoDup_concat_iff; split_all.
+        -- intros x. rewrite in_map_iff.
+          intros [pt1 [Hx Hinx]]; subst.
+          rewrite (in_map2_iff _ _ _ (Pwild, Ftrue) nil) in Hinx; wf_tac.
+          destruct Hinx as [i [Hi Hpt1]].
+          rewrite NoDup_app_iff'.
+          split_all; subst; wf_tac.
+          ++ rewrite alpha_p_aux_bnd_f_eq.
+            rewrite Forall_forall in H0.
+            apply H0; auto; wf_tac.
+          ++ intros x.
+            rewrite alpha_p_aux_bnd_f_eq.
+            intros [Hinx1 Hinx2].
+            (*Need this a lot even though it's ugly*)
+            apply alpha_p_aux_wf_aux in Hinx1; wf_tac.
+            rewrite map_snd_combine in Hinx1; wf_tac.
+            rewrite Forall_forall in H0.
+            apply H0 in Hinx2; wf_tac.
+            apply (nodup_firstn_skipn Hinx1 Hinx2); wf_tac.
+        -- intros i1 i2 d x. wf_tac.
+          rewrite !map2_nth with(d1:=(Pwild, Ftrue)) (d2:=nil); wf_tac.
+          intros [Hini1 Hini2].
+          apply in_app_or in Hini1, Hini2.
+          (*Now we get 4 cases need to show each is impossible*)
+          destruct Hini1 as [Hini1 | Hini1].
+          ++ apply alpha_p_aux_wf_aux in Hini1; wf_tac.
+            revert Hini1. wf_tac. intros Hini1.
+            apply In_firstn in Hini1.
+            destruct Hini2 as [Hini2 | Hini2].
+            ** apply alpha_p_aux_wf_aux in Hini2; wf_tac.
+              revert Hini2. wf_tac. intros Hini2.
+              apply In_firstn in Hini2.
+              apply H5.
+              apply (in_nth_concat_nodup Hini1 Hini2); wf_tac.
+            ** rewrite alpha_p_aux_bnd_f_eq in Hini2.
+              rewrite Forall_forall in H0.
+              apply H0 in Hini2; wf_tac.
+              apply In_skipn in Hini2.
+              apply H5.
+              apply (in_nth_concat_nodup Hini1 Hini2); wf_tac.
+          ++ rewrite alpha_p_aux_bnd_f_eq in Hini1.
+            rewrite Forall_forall in H0.
+            apply H0 in Hini1; wf_tac.
+            apply In_skipn in Hini1.
+            destruct Hini2 as [Hini2 | Hini2].
+            ** apply alpha_p_aux_wf_aux in Hini2; wf_tac.
+              revert Hini2; wf_tac. intros Hini2.
+              apply In_firstn in Hini2.
+              apply H5.
+              apply (in_nth_concat_nodup Hini1 Hini2); wf_tac.
+            ** rewrite alpha_p_aux_bnd_f_eq in Hini2.
+              apply H0 in Hini2; wf_tac.
+              apply In_skipn in Hini2.
+              apply H5.
+              apply (in_nth_concat_nodup Hini1 Hini2); wf_tac.
+    * intros x.
+      rewrite in_concat. intros [Hinx1 [l1 [Hinl1 Hinxl1]]].
+      apply H in Hinx1; wf_tac.
+      rewrite in_map_iff in Hinl1. destruct Hinl1 as [p1 [Hl1 Hinp1]].
+      subst.
+      rewrite in_map2_iff with(d1:=(Pwild, Ftrue))(d2:=nil) in Hinp1; wf_tac.
+      destruct Hinp1 as [i [Hi Hp1]]; subst.
+      (*And now we have to show these are distinct, will be similar*)
+      apply in_app_or in Hinxl1.
+      destruct Hinxl1 as [Hinx2 | Hinx2].
+      -- apply alpha_p_aux_wf_aux in Hinx2; wf_tac.
+        revert Hinx2; wf_tac; intros.
+        apply In_firstn in Hinx2.
+        apply in_split_lens_ith in Hinx2; wf_tac.
+        apply (nodup_firstn_skipn Hinx1 Hinx2); wf_tac.
+      -- rewrite alpha_p_aux_bnd_f_eq in Hinx2.
+        rewrite Forall_forall in H0; apply H0 in Hinx2; wf_tac.
+        apply In_skipn in Hinx2.
+        apply in_split_lens_ith in Hinx2; wf_tac.
+        apply (nodup_firstn_skipn Hinx1 Hinx2); wf_tac.
+    + (*Second part - TODO very similar to previous*)
+    intros x Hinx.
+    apply in_app_or in Hinx.
+    destruct Hinx as [Hinx | Hinx].
+    * apply H in Hinx; wf_tac.
+    * rewrite in_concat in Hinx.
+      destruct Hinx as [l1 [Hinl1 Hinxl1]].
+      rewrite in_map_iff in Hinl1.
+      destruct Hinl1 as [p1 [Hl1 Hinp1]].
+      subst.
+      rewrite in_map2_iff with (d1:=(Pwild, Ftrue))(d2:=nil) in Hinp1; wf_tac.
+      destruct Hinp1 as [i [Hi Hp1]]; subst.
+      apply in_app_or in Hinxl1.
+      destruct Hinxl1 as [Hinx | Hinx].
+      -- apply alpha_p_aux_wf_aux in Hinx; wf_tac.
+        revert Hinx; wf_tac; intros.
+        apply In_firstn in Hinx.
+        apply in_split_lens_ith in Hinx; wf_tac.
+      -- rewrite alpha_p_aux_bnd_f_eq in Hinx.
+        rewrite Forall_forall in H0; apply H0 in Hinx; wf_tac.
+        apply In_skipn in Hinx.
+        apply in_split_lens_ith in Hinx; wf_tac.
+Qed.
+
+
+(*Need to know that all patterns in constrs are valid*)
+
+(*Generalized so it works for terms and formulas*)
+Lemma alpha_p_aux_valid {A B: Type} (sub: vsymbol -> vsymbol -> A -> A)
+  (valid: A -> B -> Prop)(p: pattern) (a: A)
+  (l: list (vsymbol * string))
+  (Hnodup1: NoDup (map fst l))
+  (Hnodup2: NoDup (map snd l))
+  (sub_valid: forall a x y b,
+    valid a b ->
+    snd x = snd y ->
+    valid (sub x y a) b):
+  (forall v : vsymbol, In v (pat_fv p) -> In v (map fst l)) ->
+  (forall ty, pattern_has_type sigma p ty ->
+    pattern_has_type sigma (fst (alpha_p_aux sub p a l)) ty) /\
+  (forall b, valid a b ->
+    valid (snd (alpha_p_aux sub p a l)) b).
+Proof.
+  revert a.
+  (*revert l t Hnodup1 Hnodup2.*) induction p; simpl; auto; intros.
+  - (*Pvar*) 
+    destruct (get_assoc_list vsymbol_eq_dec l v) eqn : Ha; 
+    simpl; split; intros; auto.
+    inversion H0; subst.
+    replace (snd v) with (snd ((s, snd v))) at 2 by auto.
+    constructor; auto.
+  - (*Pconstr*)
+    split; intros.
+    + inversion H1; subst. subst sigma0.
+      assert (Hlen: 
+      Datatypes.length
+      (fst
+         ((fix alpha_ps_aux (l1 : list pattern) (y : A) {struct l1} :
+               list pattern * A :=
+             match l1 with
+             | [] => ([], y)
+             | ph :: pt =>
+                 (fst (alpha_p_aux sub ph y l)
+                  :: fst (alpha_ps_aux pt (snd (alpha_p_aux sub ph y l))),
+                 snd (alpha_ps_aux pt (snd (alpha_p_aux sub ph y l))))
+             end) ps a)) = Datatypes.length (s_args f)). {
+        rewrite <- H7. clear. revert a. induction ps; simpl; auto.
+      }
+      constructor; auto.
+      * revert H11. rewrite !Forall_forall.
+        assert (length (map (ty_subst (s_params f) vs) (s_args f)) = length ps) by wf_tac.
+        generalize dependent (map (ty_subst (s_params f) vs) (s_args f)).
+        clear -H H0.
+        revert a. induction ps; simpl; auto ; intros; destruct l0.
+        -- inversion H1.
+        -- inversion H; subst. simpl in H1. destruct H1; subst; simpl.
+          ++ apply H5; auto.
+            intros. apply H0. simpl. rewrite union_elts. left; auto.
+            specialize (H11 (a, v)); simpl in H11.
+            apply H11; left; auto.
+          ++ apply (IHps H6) with (a:=(snd (alpha_p_aux sub a a0 l))) (l:=l0); auto.
+            intros. apply H0. simpl. rewrite union_elts. right; auto.
+            intros.
+            apply H11; right; auto.
+      * rewrite Hlen, <- H7.
+        clear Hlen. clear -H12 H0 H Hnodup2. revert a.
+        (*We need a separate inductive lemma:*)
+        assert (Hinnth: forall (ps: list pattern) (j : nat) (x : vsymbol) (d : pattern) (a : A),
+        j < Datatypes.length ps ->
+        (forall v : vsymbol,
+         In v (big_union vsymbol_eq_dec pat_fv ps) -> In v (map fst l)) ->
+        In x
+          (pat_fv
+             (nth j
+                (fst
+                   ((fix alpha_ps_aux (l1 : list pattern) (y : A) {struct l1} :
+                         list pattern * A :=
+                       match l1 with
+                       | [] => ([], y)
+                       | ph :: pt =>
+                           (fst (alpha_p_aux sub ph y l)
+                            :: fst (alpha_ps_aux pt (snd (alpha_p_aux sub ph y l))),
+                           snd (alpha_ps_aux pt (snd (alpha_p_aux sub ph y l))))
+                       end) ps a)) d)) ->
+        exists v' : vsymbol, In (v', fst x) l /\ In v' (pat_fv (nth j ps Pwild))). {
+          clear.
+          induction ps; simpl; auto; intros; try lia.
+            destruct j.
+            - apply alpha_p_aux_wf_aux_gen in H1; auto.
+              intros. apply H0. rewrite union_elts. left; auto.
+            - eapply IHps; try lia; auto. 2: apply H1.
+              intros. apply H0. rewrite union_elts. right; auto.
+        }
+        intros t i j d x Hi Hj Hij [Hinx1 Hinx2].
+        apply Hinnth in Hinx1; auto.
+        apply Hinnth in Hinx2; auto.
+        destruct Hinx1 as [v1 [Hinl1 Hinv1]].
+        destruct Hinx2 as [v2 [Hinl2 Hinv2]].
+        assert (v1 = v2) by apply (nodup_snd_inj Hnodup2 Hinl1 Hinl2). 
+        subst.
+        (*This contradicts the disjointness of free vars*)
+        apply (H12 i j Pwild v2); try lia; auto.
+    + (*term goal*)
+      generalize dependent a.
+      revert H. clear - H0.
+      induction ps; simpl; auto; intros.
+      inversion H; subst.
+      apply IHps; auto.
+      * intros. apply H0. simpl. rewrite union_elts. right; auto.
+      * apply H4; auto. intros. apply H0. simpl. rewrite union_elts.
+        left; auto.
+  - (*Por case*)
+    split; intros.
+    + inversion H0; subst.
+      constructor; auto.
+      * apply IHp1; auto.
+        intros. apply H. rewrite union_elts; left; auto.
+      * apply IHp2; auto.
+        intros; apply H; rewrite union_elts; right; auto.
+      * intros x. rewrite !alpha_p_aux_wf_aux_gen'; auto;
+        try (intros; apply H; simpl; rewrite union_elts;
+          try(solve[left; auto]); right; auto).
+        setoid_rewrite H7. reflexivity.
+    + apply IHp2; auto.
+      intros. apply H. rewrite union_elts; right; auto.
+  - (*Pbind case*)
+    split; intros.
+    + inversion H0; subst. 
+      destruct (get_assoc_list vsymbol_eq_dec l v) eqn : Ha;
+      simpl; auto.
+      replace (snd v) with (snd ((s, snd v))) at 2 by auto.
+      constructor; simpl.
+      * intro. 
+        rewrite alpha_p_aux_wf_aux_gen' in H1; auto.
+        destruct H1 as [v1 [str [Hinl [Hinv1 [Hsnd Hfst]]]]];
+        simpl in *; subst.
+        apply get_assoc_list_some in Ha.
+        assert (v = v1) by apply (nodup_snd_inj Hnodup2 Ha Hinl); subst.
+        apply H4. wf_tac.
+        intros. apply H. rewrite union_elts; left; auto.
+      * apply IHp; auto. intros.
+        apply H; rewrite union_elts; left; auto.
+    + destruct (get_assoc_list vsymbol_eq_dec l v) eqn : Ha; simpl; auto.
+      apply sub_valid; auto.
+      apply IHp; auto.
+      intros. apply H. rewrite union_elts; left; auto.
+Qed.
+
+
+Lemma alpha_p_aux_valid_t (p: pattern) (t: term)
+  (l: list (vsymbol * string))
+  (Hnodup1: NoDup (map fst l))
+  (Hnodup2: NoDup (map snd l)):
+  (forall v : vsymbol, In v (pat_fv p) -> In v (map fst l)) ->
+  (forall ty, pattern_has_type sigma p ty ->
+    pattern_has_type sigma (fst (alpha_p_aux sub_t p t l)) ty) /\
+  (forall ty, term_has_type sigma t ty ->
+    term_has_type sigma (snd (alpha_p_aux sub_t p t l)) ty).
+Proof.
+  apply alpha_p_aux_valid; auto.
+  apply sub_t_valid.
+Qed.
+
+Lemma alpha_p_aux_valid_f (p: pattern) (f: formula)
+  (l: list (vsymbol * string))
+  (Hnodup1: NoDup (map fst l))
+  (Hnodup2: NoDup (map snd l)):
+  (forall v : vsymbol, In v (pat_fv p) -> In v (map fst l)) ->
+  (forall ty, pattern_has_type sigma p ty ->
+    pattern_has_type sigma (fst (alpha_p_aux sub_f p f l)) ty) /\
+  (valid_formula sigma f ->
+    valid_formula sigma (snd (alpha_p_aux sub_f p f l))).
+Proof.
+  intros Hinfv.
+  pose proof (alpha_p_aux_valid sub_f 
+    (fun f' (u: unit) => valid_formula sigma f') 
+      p f l Hnodup1 Hnodup2);
+  split; apply H; auto; try(intros; apply sub_f_valid; auto).
+  exact tt.
+Qed.
+
+(*Part 2: [alpha_t_aux] and [alpha_f_aux] form well-typed
+  terms and formulas*)
+Lemma alpha_aux_valid (t: term) (f: formula):
+  (forall (l: list string) (ty: vty)
+    (Hnodup: NoDup l)
+    (Hlenl: length l = length (bnd_t t)),
+    term_has_type sigma t ty ->
+    term_has_type sigma (alpha_t_aux t l) ty) /\
+  (forall (l: list string)
+    (Hnodup: NoDup l)
+    (Hlenl: length l = length (bnd_f f)),
+    valid_formula sigma f ->
+    valid_formula sigma (alpha_f_aux f l)).
+Proof.
+  revert t f.
+  apply term_formula_ind; simpl; auto; simpl; intros.
+  - (*Tfun*)
+    inversion H0; subst. constructor; auto.
+    wf_tac. revert H11 H.
+    rewrite !Forall_forall; intros.
+    rewrite in_combine_iff in H1; wf_tac.
+    destruct H1 as [i [Hi Hx]].
+    revert Hi; wf_tac.
+    specialize (Hx tm_d vty_int); subst; simpl.
+    rewrite map2_nth with(d1:=tm_d) (d2:=nil); wf_tac.
+    apply H; wf_tac.
+    rewrite map_nth_inbound with(d2:=vty_int); try lia.
+    apply (H11 (nth i l1 tm_d, 
+      (ty_subst (s_params f1) l (nth i (s_args f1) vty_int)))).
+    rewrite in_combine_iff; wf_tac.
+    exists i. split; auto. intros.
+    f_equal.
+    + apply nth_indep; auto.
+    + rewrite map_nth_inbound with (d2:=vty_int); auto. lia.
+  - (*Tlet*) destruct l; auto; simpl.
+    inversion H1; subst.
+    inversion Hnodup; subst.
+    wf_tac. inversion Hlenl.
+    constructor.
+    + apply H; wf_tac.
+    + apply sub_t_valid; auto. apply H0; wf_tac.
+  - (*Tif*) inversion H2; subst.
+    constructor; auto.
+    apply H; wf_tac.
+    apply H0; wf_tac.
+    apply H1; wf_tac.
+  - (*Tmatch*)
+    assert (Hsum: sum (map
+      (fun x : pattern * term =>
+      Datatypes.length (pat_fv (fst x)) + Datatypes.length (bnd_t (snd x)))
+      ps) = Datatypes.length (skipn (Datatypes.length (bnd_t tm)) l)). {
+        wf_tac. rewrite Hlenl,length_concat, 
+      map_map, minus_plus. f_equal. apply map_ext_in_iff; intros.
+      rewrite app_length; auto.
+    }
+    inversion H1; subst.
+    constructor.
+    + apply H; auto; wf_tac.
+    + intros x.
+      rewrite in_map2_iff with(d1:=(Pwild, tm_d))(d2:=nil); wf_tac.
+      intros [i [Hi Hx]]; subst.
+      apply alpha_p_aux_valid_t; wf_tac.
+      apply H7; wf_tac.
+    + intros x.
+      rewrite in_map2_iff with(d1:=(Pwild, tm_d))(d2:=nil); wf_tac.
+      intros [i [Hi Hx]]; subst.
+      apply alpha_p_aux_valid_t; wf_tac.
+      rewrite Forall_forall in H0. apply H0; wf_tac.
+      apply H9; wf_tac.
+    + rewrite null_map2; auto; wf_tac.
+  - (*Teps*)
+    destruct l; inversion Hlenl.
+    inversion H0; subst.
+    replace (snd v) with (snd (s, snd v)) at 3 by auto.
+    constructor; auto.
+    apply sub_f_valid; auto. inversion Hnodup. apply H; wf_tac.
+  - (*Fpred*)
+    inversion H0; subst.
+    constructor; auto; wf_tac.
+    revert H9 H.
+    rewrite !Forall_forall; intros.
+    rewrite in_combine_iff in H1; wf_tac.
+    destruct H1 as [i [Hi Hx]].
+    revert Hi; wf_tac.
+    specialize (Hx tm_d vty_int); subst; simpl.
+    rewrite map2_nth with(d1:=tm_d) (d2:=nil); wf_tac.
+    apply H; wf_tac.
+    rewrite map_nth_inbound with(d2:=vty_int); try lia.
+    apply (H9 (nth i tms tm_d, 
+      (ty_subst (p_params p) tys (nth i (p_args p) vty_int)))).
+    rewrite in_combine_iff; wf_tac.
+    exists i. split; auto. intros.
+    f_equal.
+    + apply nth_indep; auto.
+    + rewrite map_nth_inbound with (d2:=vty_int); auto. lia.
+  - (*Fquant*)
+    destruct l; inversion Hlenl.
+    inversion H0; subst.
+    constructor; auto.
+    apply sub_f_valid; auto.
+    apply H; auto. inversion Hnodup; auto.
+  - (*Feq*)
+    inversion H1; subst.
+    constructor; [apply H | apply H0]; wf_tac.
+  - (*Fbinop*)
+    inversion H1; subst.
+    constructor; [apply H | apply H0]; wf_tac.
+  - (*Fnot*)
+    inversion H0; subst.
+    constructor. apply H; wf_tac.
+  - (*Flet*)
+    destruct l; inversion Hlenl; simpl.
+    inversion H1; subst.
+    inversion Hnodup; subst.
+    constructor; [apply H | apply sub_f_valid]; wf_tac.
+    apply H0; wf_tac.
+  - (*Fif*)
+    inversion H2; subst.
+    constructor; [apply H | apply H0 | apply H1]; wf_tac.
+  - (*Fmatch*)
+    assert (Hsum: sum (map
+      (fun x : pattern * formula =>
+      Datatypes.length (pat_fv (fst x)) + Datatypes.length (bnd_f (snd x)))
+      ps) = Datatypes.length (skipn (Datatypes.length (bnd_t tm)) l)). {
+        wf_tac. rewrite Hlenl,length_concat, 
+      map_map, minus_plus. f_equal. apply map_ext_in_iff; intros.
+      rewrite app_length; auto.
+    }
+    inversion H1; subst.
+    constructor.
+    + apply H; auto; wf_tac.
+    + rewrite Forall_forall; intros x.
+      rewrite in_map2_iff with(d1:=(Pwild, Ftrue))(d2:=nil); wf_tac.
+      intros [i [Hi Hx]]; subst.
+      apply alpha_p_aux_valid_f; wf_tac.
+      rewrite Forall_forall in H7;
+      apply H7; wf_tac.
+    + rewrite Forall_forall; intros x.
+      rewrite in_map2_iff with(d1:=(Pwild, Ftrue))(d2:=nil); wf_tac.
+      intros [i [Hi Hx]]; subst.
+      apply alpha_p_aux_valid_f; wf_tac.
+      rewrite Forall_forall in H0. apply H0; wf_tac.
+      rewrite Forall_forall in H8; apply H8; wf_tac.
+    + rewrite null_map2; auto; wf_tac.
+Qed.
+
+(*Finally, we need to prove that the [alpha] functions
+  do not change the meaning of the term/formula (since we
+  only rename bound variables)*)
